chore: lean refactor (#201)

lean/privacy/notes/canceled_notes.lean
@@ -1,94 +1,164 @@
 import privacy.utils
 import privacy.actions
 import privacy.notes.notes
+import privacy.notes.note_implies
 import privacy.subchannels.subchannels
 
 def note_canceled (crypto: Crypto) (m: Memory) (c token i₀ i₁ kbob: ℕ) : Prop :=
   m .Nullifiers [crypto.hash [c, token, i₀, i₁, kbob]] ≠ 0
 
--- Once a note is canceled, it stays canceled.
-theorem note_canceled_monotone
-    {crypto: Crypto} {rm: ReachableMemory crypto} {action: Action}
-    (success: (run_action crypto action rm.m).success)
-    (h: note_canceled crypto rm.m c token i₀ i₁ kbob) :
-    note_canceled crypto (rm.add action success) c token i₀ i₁ kbob := by
-  unfold note_canceled
+structure CancelImplies₀
+    {crypto: Crypto} (rm: ReachableMemory crypto) (inp: CancelNoteInput) where
+  h_action: .CancelNote inp ∈ rm.actions
+  (addralice kalice r_create amount_create: ℕ)
+  amount_nz: inp.amount ≠ 0
+  h_kbob: inp.kbob ∈ crypto.PrivateKeys
+
+abbrev CancelImplies₀.inp_create
+    {crypto: Crypto} {rm: ReachableMemory crypto} {inp: CancelNoteInput}
+    (self: CancelImplies₀ rm inp) : CreateNoteInput :=
+  ⟨self.addralice, self.kalice, inp.addrbob, crypto.priv_to_pub inp.kbob, inp.token, inp.i₀, inp.i₁, self.r_create, self.amount_create⟩
+
+structure CancelImplies
+    {crypto: Crypto} (rm: ReachableMemory crypto) (inp: CancelNoteInput)
+    extends CancelImplies₀ rm inp where
+  h_note_canceled: note_canceled crypto rm.m inp.c inp.token inp.i₀ inp.i₁ inp.kbob
+  note_created: NoteImplies rm (toCancelImplies₀.inp_create)
+  h_c: toCancelImplies₀.inp_create.c crypto = inp.c
+
+theorem CancelImplies.h_note_exists
+    {crypto: Crypto} {rm: ReachableMemory crypto} {inp: CancelNoteInput}
+    (cancel_imp: CancelImplies rm inp) :
+    rm.m .Notes [inp.note_id crypto, 0] ≠ 0 := by
+  have := cancel_imp.note_created.h_note_exists
+  unfold note_exists CreateNoteInput.note_id at this
+  simp only [cancel_imp.h_c] at this
+  exact this
+
+theorem CancelImplies.h_kbob'
+    {crypto: Crypto} {rm: ReachableMemory crypto} {inp: CancelNoteInput}
+    (cancel_imp: CancelImplies rm inp) :
+    cancel_imp.note_created.subchannel.channel.kbob = inp.kbob := by
+  apply crypto.priv_to_pub_inj cancel_imp.note_created.subchannel.channel.kbob.prop cancel_imp.h_kbob
+  rw [cancel_imp.note_created.h_Kbob]
+
+theorem CancelImplies.next
+    {crypto: Crypto} {rm: ReachableMemory crypto} {inp: CancelNoteInput}
+    {action: Action} (success: (run_action crypto action rm.m).success)
+    (cancel_imp: CancelImplies rm inp) :
+    Nonempty (CancelImplies (rm.add action success) inp) := by
+  let res : CancelImplies₀ (rm.add action success) inp := {
+    h_action := by simp [cancel_imp.h_action]
+    addralice := cancel_imp.addralice
+    kalice := cancel_imp.kalice
+    r_create := cancel_imp.r_create
+    amount_create := cancel_imp.amount_create
+    amount_nz := cancel_imp.amount_nz
+    h_kbob := cancel_imp.h_kbob
+  }
+
   cases action
-  case CancelNote inp =>
+  case CancelNote inp' =>
+    let info := cancel_note_info crypto inp' rm success
+    have : inp.nullifier crypto ≠ inp'.nullifier crypto := by
+      by_contra h
+      have := cancel_imp.h_note_canceled
+      rw [note_canceled, ←CancelNoteInput.nullifier, h] at this
+      exact this info.nullifier_didnt_exist
+    exact ⟨{
+      toCancelImplies₀ := res,
+      h_note_canceled := by
+        rw [ReachableMemory.add_m, run_action, ←info.h_m', note_canceled]
+        rw [info.no_change _ _ (by simp [this])]
+        exact cancel_imp.h_note_canceled
+      note_created := Nonempty.some (cancel_imp.note_created.next success)
+      h_c := cancel_imp.h_c
+    }⟩
+
+  all_goals exact ⟨{
+    toCancelImplies₀ := res,
+    h_note_canceled := cancel_imp.h_note_canceled
+    note_created := Nonempty.some (cancel_imp.note_created.next success)
+    h_c := cancel_imp.h_c
+  }⟩
+
+theorem CancelImplies.from_action
+    {crypto: Crypto} {rm: ReachableMemory crypto} {inp: CancelNoteInput}
+    (h: .CancelNote inp ∈ rm.actions) :
+    Nonempty (CancelImplies rm inp) := by
+  revert rm
+  apply ReachableMemory.induction
+  case inv₀ => intro h; contradiction
+
+  intro action rm ih success h
+  cases h
+
+  case head =>
     let info := cancel_note_info crypto inp rm success
-    rw [ReachableMemory.add_m, run_action, ←info.h_m']
-    by_cases h_is_same : crypto.hash [c, token, i₀, i₁, kbob] = inp.nullifier crypto
-    case pos =>
-      simp [h_is_same, info.memory_diff₀]
-    case neg =>
-      rw [info.no_change _ _ (by simp [h_is_same])]
-      exact h
+    have ⟨inp_create, note_imp, h_note_id⟩ := NoteImplies.from_note_exists info.r_ne_zero
+    have ⟨addralice, ⟨subchannel_imp⟩⟩ := SubchannelImplies.from_subchannel_hash_exists info.subchannel_exists
 
-  repeat exact h
+    let res : CancelImplies₀ (rm.add (.CancelNote inp) success) inp := {
+      h_action := by simp
+      addralice := inp_create.addralice
+      kalice := inp_create.kalice
+      r_create := inp_create.r
+      amount_create := inp_create.amount
+      amount_nz := info.amount_ne_zero
+      h_kbob := info.kbob_private_key
+    }
 
--- Canceled note must exist.
-theorem canceled_note_implies_exists
+    have h_inp_create: inp.c = inp_create.c crypto ∧ inp_create = res.inp_create := by
+      unfold CancelImplies₀.inp_create
+      have := crypto.h_hash (Eq.symm h_note_id)
+      injections
+      simp only [*, true_and]
+
+      have := calc subchannel_imp.channel.c
+        _ = inp.c := by simp [subchannel_imp.h_c]
+        _ = inp_create.c crypto := by assumption
+      have ⟨_, _, h_addrbob, h_kbob⟩ := subchannel_imp.channel.same_c this
+      simp only [CancelNoteInput.Kbob] at h_addrbob h_kbob
+      rw [←h_addrbob, ←h_kbob]
+
+    exact ⟨{
+      toCancelImplies₀ := res,
+      h_note_canceled := by rw [rm.add_m, run_action, ←info.h_m', note_canceled, info.memory_diff₀]; simp
+      note_created := h_inp_create.2 ▸ note_imp.next success |>.some
+      h_c := by simp [h_inp_create]
+    }⟩
+
+  case tail h => exact (ih h |>.some).next success
+
+theorem CancelImplies.from_note_canceled
     {crypto: Crypto} {rm: ReachableMemory crypto} {c token i₀ i₁ kbob: ℕ}
-    (h_note_canceled: note_canceled crypto rm c token i₀ i₁ kbob) :
-    note_exists rm (crypto.hash [c, token, i₀, i₁]) := by
+    (h: note_canceled crypto rm c token i₀ i₁ kbob) :
+    ∃ addrbob amount, Nonempty (CancelImplies rm ⟨c, addrbob, kbob, token, i₀, i₁, amount⟩) := by
   revert rm
   apply ReachableMemory.induction
   case inv₀ => intro h; trivial
 
-  intro action rm ih success h_note_canceled
+  intro action rm ih success h
   cases action
   case CancelNote inp =>
-    dsimp only [note_canceled, note_exists] at h_note_canceled ⊢
     let info := cancel_note_info crypto inp rm success
-    by_cases h_is_same : crypto.hash [c, token, i₀, i₁] = inp.note_id crypto ∧ kbob = inp.kbob
+    have ⟨kalice, ⟨subchannel_imp⟩⟩ := SubchannelImplies.from_subchannel_hash_exists info.subchannel_exists
+    by_cases h_is_same : crypto.hash [c, token, i₀, i₁, kbob] = inp.nullifier crypto
     case pos =>
-      rw [ReachableMemory.add_m, run_action, ←info.h_m', h_is_same.1, info.no_change _ _ (by simp)]
-      use info.r_ne_zero
+      use inp.addrbob, inp.amount
+      have := crypto.h_hash h_is_same
+      repeat injection this with _ this
+      apply CancelImplies.from_action
+      simp [*]
     case neg =>
-      have : crypto.hash [c, token, i₀, i₁, kbob] ≠ CancelNoteInput.nullifier crypto inp := by
-        by_contra h₀
-        apply crypto.h_hash at h₀
-        repeat injection h₀ with _ h₀
-        simp [*] at h_is_same
-      rw [ReachableMemory.add_m, run_action, ←info.h_m', info.no_change _ _ (by simp [this])] at h_note_canceled
-      exact note_exists_monotone success (ih h_note_canceled)
+      rw [note_canceled, ReachableMemory.add_m, run_action, ←info.h_m'] at h
+      rw [info.no_change _ _ (by simp [h_is_same])] at h
+      have ⟨addrbob, amount, ⟨cancel_imp⟩⟩ := ih h
+      exact ⟨addrbob, amount, cancel_imp.next success⟩
 
-  case CreateNote inp =>
-    exact note_exists_monotone success (ih h_note_canceled)
-
-  case OpenDeposit inp =>
-    exact note_exists_monotone success (ih h_note_canceled)
-
-  repeat exact ih h_note_canceled
-
--- If a note was canceled, kbob must be a valid private key.
-theorem canceled_note_implies_kbob_private_key
-    {crypto: Crypto} {rm: ReachableMemory crypto} {c token i₀ i₁ kbob: ℕ}
-    (h_note_canceled: note_canceled crypto rm c token i₀ i₁ kbob) :
-    kbob ∈ crypto.PrivateKeys := by
-  revert rm
-  apply ReachableMemory.induction
-  case inv₀ => intro h_note_canceled; trivial
-
-  intro action rm ih success h_note_canceled
-  cases action
-  case CancelNote inp =>
-    dsimp only [note_canceled] at h_note_canceled
-    let info := cancel_note_info crypto inp rm success
-    by_cases h_is_same : crypto.hash [c, token, i₀, i₁] = inp.note_id crypto ∧ kbob = inp.kbob
-    case pos =>
-      simp only [h_is_same]
-      exact info.kbob_private_key
-    case neg =>
-      have : crypto.hash [c, token, i₀, i₁, kbob] ≠ CancelNoteInput.nullifier crypto inp := by
-        by_contra h₀
-        apply crypto.h_hash at h₀
-        repeat injection h₀ with _ h₀
-        simp [*] at h_is_same
-      rw [ReachableMemory.add_m, run_action, ←info.h_m', info.no_change _ _ (by simp [this])] at h_note_canceled
-      exact ih h_note_canceled
-
-  repeat exact ih h_note_canceled
+  all_goals
+    have ⟨addrbob, amount, ⟨cancel_imp⟩⟩ := ih h
+    exact ⟨addrbob, amount, cancel_imp.next success⟩
 
 def cancel_note_actions (crypto: Crypto) (rm: ReachableMemory crypto) : List CancelNoteInput :=
   rm.actions.filterMap filter_CancelNote
@@ -100,119 +170,27 @@ theorem cancel_note_actions_add
     inp :: cancel_note_actions crypto rm := by
   simp [cancel_note_actions]
 
--- Note is canceled ↔ there's a CancelNote action that corresponds to the note_id.
-theorem cancel_note_actions_iff_note_canceled {crypto: Crypto} {rm: ReachableMemory crypto} {c token i₀ i₁ kbob: ℕ} :
-    note_canceled crypto rm c token i₀ i₁ kbob ↔
-    ∃ inp, inp ∈ cancel_note_actions crypto rm ∧
-      inp.note_id crypto = crypto.hash [c, token, i₀, i₁] ∧
-      inp.kbob = kbob := by
-  revert rm
-  apply ReachableMemory.induction
-  case inv₀ =>
-    constructor
-    · intro h; contradiction
-    · intro h; obtain ⟨inp, h₀, h₁⟩ := h; contradiction
+theorem CancelImplies.in_cancel_note_actions
+    {crypto: Crypto} {rm: ReachableMemory crypto} {inp: CancelNoteInput}
+    (note_imp: CancelImplies rm inp) :
+    inp ∈ cancel_note_actions crypto rm := by
+  simp [cancel_note_actions]
+  use .CancelNote inp
+  simp [note_imp.h_action]
 
-  intro action rm ih success
-  cases action
-  case CancelNote inp =>
-    let info := cancel_note_info crypto inp rm success
-    rw [cancel_note_actions_add]
-    simp only [List.mem_cons, exists_eq_or_imp]
-
-    by_cases h_is_same : crypto.hash [c, token, i₀, i₁] = inp.note_id crypto ∧ inp.kbob = kbob
-    case pos =>
-      constructor
-      · intro h'
-        apply Or.inl
-        simp [h_is_same]
-      · intro h'
-        have := h_is_same.1
-        apply crypto.h_hash at this
-        repeat injection this with _ this
-
-        rw [ReachableMemory.add_m, run_action, ←info.h_m', note_canceled]
-        simp only [*]
-        simp [←h_is_same.2, info.memory_diff₀]
-    case neg =>
-      constructor
-      · intro h'
-        by_cases h_canceled_before: note_canceled crypto rm.m c token i₀ i₁ kbob
-        case pos =>
-          obtain ⟨inp, ih⟩ := ih.1 h_canceled_before
-          apply Or.inr
-          use inp
-        case neg =>
-          apply Or.inl
-          rw [ReachableMemory.add_m, run_action, ←info.h_m', note_canceled, info.no_change _ _ (by
-            by_contra h₀
-            simp only [CancelNoteInput.nullifier, Prod.mk.injEq, List.cons.injEq, and_true,
-              true_and] at h₀
-            apply crypto.h_hash at h₀
-            repeat injection h₀ with _ h₀
-            simp [*] at h_is_same
-          )] at h'
-          contradiction
-      ·
-        intro h'
-        cases h'
-        case inl h' =>
-          have := crypto.h_hash (Eq.symm h'.1)
-          injections
-          rw [ReachableMemory.add_m, run_action, ←info.h_m', note_canceled]
-          simp [*]
-          simp [←h'.2, info.memory_diff₀]
-        case inr h' =>
-          exact note_canceled_monotone success (ih.2 h')
-
-  repeat exact ih
-
-theorem note_cancel_action_implies
+theorem CancelImplies.from_cancel_note_actions
     {crypto: Crypto} {rm: ReachableMemory crypto} {inp: CancelNoteInput}
     (h: inp ∈ cancel_note_actions crypto rm) :
-    (∃ addralice kalice, inp.c = crypto.hash [addralice, kalice, inp.addrbob, inp.Kbob crypto]) ∧
-    inp.kbob ∈ crypto.PrivateKeys ∧
-    inp.amount ≠ 0 ∧
-    note_canceled crypto rm inp.c inp.token inp.i₀ inp.i₁ inp.kbob := by
-  revert rm
-  apply ReachableMemory.induction
-  case inv₀ => intro h; trivial
-
-  intro action rm ih success h
-  cases action
-  case CancelNote inp' =>
-    rw [cancel_note_actions_add, List.mem_cons] at h
-    cases h
-
-    case inl h =>
-      rw [h]
-      let info := cancel_note_info crypto inp' rm success
-
-      exact ⟨
-        subchannel_hash_exists_implies_hash info.subchannel_exists,
-        info.kbob_private_key,
-        info.amount_ne_zero,
-        by
-          rw [ReachableMemory.add_m, run_action, ←info.h_m', note_canceled, info.memory_diff₀]
-          simp
-      ⟩
-    case inr h =>
-      have ⟨ih₀, ih₁, ih₂, ih₃⟩ := ih h
-      exact ⟨ih₀, ih₁, ih₂, note_canceled_monotone success ih₃⟩
-
-  repeat exact ih h
+    Nonempty (CancelImplies rm inp) := by
+  simp only [cancel_note_actions, List.mem_filterMap, filter_CancelNote_some, exists_eq_right] at h
+  exact CancelImplies.from_action h
 
 theorem note_canceled_monotone_extends
     {crypto: Crypto} {rm rm': ReachableMemory crypto}
     (h_extends: rm'.extends rm)
     (h: note_canceled crypto rm c token i₀ i₁ kbob) :
     note_canceled crypto rm' c token i₀ i₁ kbob := by
-  apply cancel_note_actions_iff_note_canceled.2
-  apply cancel_note_actions_iff_note_canceled.1 at h
-  obtain ⟨inp, h⟩ := h
-  use inp
-  refine ⟨?_, h.2⟩
-  obtain ⟨ℓ, h_extends⟩ := h_extends
-  rw [cancel_note_actions, ←h_extends]
-  rw [List.filterMap_append, List.mem_append, List.mem_filterMap]
-  exact Or.inr h.1
+  have ⟨addrbob, amount, ⟨cancel_imp⟩⟩ := CancelImplies.from_note_canceled h
+  have ⟨ℓ, h_extends⟩ := h_extends
+  have := h_extends ▸ (List.mem_append (s:=ℓ)).2 (Or.inr cancel_imp.h_action)
+  exact (CancelImplies.from_action this |>.some).h_note_canceled
