lean/privacy/compliance/all_notes.lean
@@ -35,55 +35,13 @@ theorem scan_all_notes_iff {crypto: Crypto} {rm: ReachableMemory crypto} {sn: Sc
     use ⟨⟨addralice, kalice⟩, h₀⟩, List.mem_attach _ ⟨_, h₀⟩, h₁
 
 -- All notes can be retrieved given the compliance private key.
-theorem all_notes_are_discoverable {crypto: Crypto} {rm: ReachableMemory crypto} {note_id: ℕ}
-  (h: note_exists rm note_id) :
-  ∃ sn ∈ scan_all_notes (.from rm),
-    note_id = sn.note_id crypto ∧
-    ∃ (addralice kalice addrbob: ℕ) (kbob: crypto.PrivateKeys),
-      sn.c = crypto.hash [addralice, kalice, addrbob, crypto.priv_to_pub kbob] ∧
-      (addralice, kalice) ∈ scan_users crypto rm.events ∧
-      (addrbob, ↑kbob) ∈ scan_users crypto rm.events := by
-  obtain ⟨addrbob, kbob, sn, h₀, h₁, h_channel_exists, ⟨addralice, kalice, h₃⟩⟩ := note_exists_implies_for_recipient h
-
-  have ⟨addralice', addrbob', Kbob, h_channel_exists⟩ := h_channel_exists
-  have ⟨⟨kalice', h_sn_c, h_public_keys_alice⟩, ⟨kbob', h_Kbob, h_public_keys_bob⟩⟩ := channel_exists_implies_hash h_channel_exists
-
-  have ⟨h_addrbob, h_kbob⟩ : addrbob = addrbob' ∧ kbob = kbob' := by
-    rw [h₃] at h_sn_c
-    have := crypto.h_hash h_sn_c
-    injections
-    simp only [true_and, *]
-    apply Subtype.coe_inj.1
-    apply crypto.priv_to_pub_inj (by simp) (by simp)
-    simp [*]
-
-  rw [h_Kbob, ←h_kbob] at h_public_keys_bob
-  have h_public_keys_bob' := h_public_keys_bob ▸ crypto.zero_not_public_key kbob
-  have h_public_keys_alice' := h_public_keys_alice ▸ crypto.zero_not_public_key kalice'
-
-  have ⟨inp_alice, h_inp_in_actions_alice, h_inp_alice₀, h_inp_alice₁, h_kalice_valid⟩ := public_key_implies h_public_keys_alice'
-  have ⟨inp_bob, h_inp_in_actions_bob, h_inp_bob₀, h_inp_bob₁, h_kbob_valid⟩ := public_key_implies h_public_keys_bob'
-
-  rw [h_public_keys_bob] at h_inp_bob₁
-  rw [h_public_keys_alice] at h_inp_alice₁
-
-  refine ⟨sn, ?_, h₁, ?_⟩
-
-  · rw [scan_all_notes_iff]
-    refine ⟨addrbob, kbob, ?_, h₀⟩
-    rw [h_addrbob]
-    rw [←h_inp_bob₀, crypto.priv_to_pub_inj (by simp) h_kbob_valid h_inp_bob₁]
-    exact register_implies_scan_users h_inp_in_actions_bob
-  · use addralice, kalice, addrbob, kbob
-    rw [h_addrbob]
-    rw [←h_inp_bob₀, crypto.priv_to_pub_inj (by simp) h_kbob_valid h_inp_bob₁]
-    refine ⟨?_, ?_, ?_⟩
-    · rw [h₃, h_inp_bob₁]; simp [*]
-    · have : addralice = addralice' ∧ kalice = kalice' := by
-        rw [h₃] at h_sn_c
-        apply crypto.h_hash at h_sn_c
-        injections
-        simp [*]
-      simp only [this, ←h_inp_alice₀, crypto.priv_to_pub_inj (by simp) h_kalice_valid h_inp_alice₁]
-      exact register_implies_scan_users h_inp_in_actions_alice
-    · exact register_implies_scan_users h_inp_in_actions_bob
+theorem NoteImplies.scan_all_notes {crypto: Crypto} {rm: ReachableMemory crypto} {inp: CreateNoteInput}
+  (note_imp: NoteImplies rm inp) :
+  inp.to_scanned_note crypto ∈ scan_all_notes (.from rm) := by
+  rw [scan_all_notes_iff]
+  exact ⟨
+    inp.addrbob,
+    note_imp.subchannel.channel.kbob,
+    note_imp.subchannel.channel.bob_registered.scan,
+    note_imp.scan_for_recipient
+  ⟩
